filled in the proof of associativity for the new `part` operator

heap2.lean
@@ -1,4 +1,5 @@
 import separation.heap
+import util.meta.tactic.ite
 
 universes u
 
@@ -6,7 +7,7 @@ section classical
 
 local attribute [instance] classical.prop_decidable
 
-noncomputable def part_  : option heap → option heap → option heap
+noncomputable def part  : option heap → option heap → option heap
 | (some hp₀) (some hp₁) :=
 if h : hp₀ ## hp₁
 then some $ part' hp₀ hp₁
@@ -19,64 +20,162 @@ end classical
 lemma some_part'
   (hp₀ hp₁ : heap)
   (h : hp₀ ## hp₁)
-: some (part' hp₀ hp₁) = part_ (some hp₀) (some hp₁) :=
-by { simp [part_,bind,option.bind,dif_pos, h], }
+: some (part' hp₀ hp₁) = part (some hp₀) (some hp₁) :=
+by { simp [part,bind,option.bind,dif_pos, h], }
 
 @[simp]
-lemma heap_emp_part_
+lemma heap_emp_part
   (hp : heap)
-: part_ (some heap.emp) (some hp) = some hp :=
-sorry
+: part (some heap.emp) (some hp) = some hp :=
+by simp [part]
 
 @[simp]
-lemma part__heap_emp
+lemma part_heap_emp
   (hp : heap)
-: part_ (some hp) (some heap.emp) = some hp :=
-sorry
+: part (some hp) (some heap.emp) = some hp :=
+by simp [part]
 
-lemma part__assoc
+namespace tactic.interactive
+
+open tactic tactic.interactive (ite_cases)
+open lean lean.parser interactive interactive.types
+
+meta def try_then (x y : tactic unit) : tactic unit :=
+focus1 $
+do (some ()) ← try_core x | tactic.skip,
+   tactic.all_goals y
+
+meta def expand_part_ite : tactic unit :=
+do tactic.try `[ dsimp [part] ],
+   tactic.reflexivity <|> try_then (ite_cases `h) expand_part_ite
+
+meta def break_disjoint_asm_symm (l : expr)
+: tactic unit :=
+do t ← infer_type l,
+   match t with
+    | `(%%h₀ ## (%%h₁ : heap)) :=
+      do h ← get_unused_name `h,
+         to_expr ``(disjoint_symm %%l) >>= note h none,
+         return ()
+    | _ :=
+         fail $ format! "expecting {l} of the form _ ## _"
+   end
+
+meta def break_disjoint_asm_r (l : expr)
+: tactic (list expr) :=
+do t ← infer_type l,
+   match t with
+    | `(%%h₀ ## part' %%h₁ %%h₂ %%h₃) :=
+      do h ← get_unused_name `h,
+         r ← to_expr ``(disjoint_of_disjoint_part'_right _ %%l) >>= note h none,
+         h ← get_unused_name `h,
+         r' ← to_expr ``(disjoint_of_disjoint_part'_left _ %%l) >>= note h none,
+         try (tactic.clear l),
+         return [r,r']
+    | _ :=
+         fail $ format! "expecting {l} of the form _ ## _"
+   end
+meta def break_disjoint_asm_l (l : expr)
+: tactic (list expr) :=
+do t ← infer_type l,
+   match t with
+    | `(part' %%h₁ %%h₂ %%h₃ ## %%h₀) :=
+      do h ← get_unused_name `h,
+         r ← to_expr ``(disjoint_of_part'_disjoint_right _ %%l) >>= note h none,
+         h ← get_unused_name `h,
+         r' ← to_expr ``(disjoint_of_part'_disjoint_left _ %%l) >>= note h none,
+         try (tactic.clear l),
+         return [r,r']
+    | _ :=
+         break_disjoint_asm_r l
+   end
+
+meta def break_disjoint_asm'
+: expr → tactic unit
+| l :=
+do xs ← break_disjoint_asm_l l,
+   xs.for_each (try ∘ break_disjoint_asm')
+
+meta def break_disjoint_asm (l : parse ident)
+: tactic (list expr) :=
+do get_local l >>= break_disjoint_asm_l
+
+meta def break_disjoint_asms
+: tactic unit :=
+do ls ← local_context,
+   ls.for_each (try ∘ break_disjoint_asm'),
+   ls ← local_context,
+   ls.for_each (try ∘ break_disjoint_asm_symm)
+
+meta def contradict_asm
+: tactic unit :=
+do ls ← local_context,
+   ls.any_of (λ e,
+     do `(¬ %%t) ← infer_type e | failed ,
+         exfalso, tactic.apply e, tactic.clear e)
+
+meta def prove_disjoint'
+: tactic unit :=
+    assumption
+<|> (`[ apply part'_disjoint ] ; assumption )
+<|> (`[ apply disjoint_part' ] ; assumption )
+<|> failed
+
+meta def prove_disjoint
+: tactic unit :=
+do contradict_asm,
+   break_disjoint_asms,
+   prove_disjoint'
+
+end tactic.interactive
+
+lemma part_assoc
   (a b c : option heap)
-: part_ (part_ a b) c = part_ a (part_ b c) :=
-sorry
+: part (part a b) c = part a (part b c) :=
+begin
+  cases a ; cases b ; cases c
+  ; expand_part_ite,
+   all_goals { prove_disjoint <|> rw part'_assoc },
+end
 
-lemma part__comm
+lemma part_comm
   (a b : option heap)
-: part_ a b = part_ b a :=
+: part a b = part b a :=
 sorry
 
-instance : is_associative (option heap) part_ :=
-⟨ part__assoc ⟩
-instance : is_commutative (option heap) part_ :=
-⟨ part__comm ⟩
+instance : is_associative (option heap) part :=
+⟨ part_assoc ⟩
+instance : is_commutative (option heap) part :=
+⟨ part_comm ⟩
 
-lemma disjoint_of_is_some_part_
+lemma disjoint_of_is_some_part
   {hp₀ hp₁ : heap}
-  (h : (part_ (some hp₀) (some hp₁)).is_some)
+  (h : (part (some hp₀) (some hp₁)).is_some)
 : hp₀ ## hp₁ :=
 sorry
 
-lemma disjoint_of_part__eq_some
+lemma disjoint_of_part_eq_some
   {hp₀ hp₁ hp₂ : heap}
-  (h : some hp₂ = (part_ (some hp₀) (some hp₁)))
+  (h : some hp₂ = (part (some hp₀) (some hp₁)))
 : hp₀ ## hp₁ :=
 sorry
 
-lemma eq_part'_of_some_eq_part_
+lemma eq_part'_of_some_eq_part
   (hp₀ hp₁ hp : heap)
-  (h : some hp = part_ (some hp₀) (some hp₁))
-: hp = part' hp₀ hp₁ (disjoint_of_part__eq_some h) :=
+  (h : some hp = part (some hp₀) (some hp₁))
+: hp = part' hp₀ hp₁ (disjoint_of_part_eq_some h) :=
 by { apply @option.no_confusion _ _ (some hp) (some _) _ id,
      simp [h], }
 
-lemma is_some_of_is_some_part__right
+lemma is_some_of_is_some_part_right
   (hp₀ : option heap) {hp₁ : option heap}
-  (h : (part_ hp₀ hp₁).is_some)
+  (h : (part hp₀ hp₁).is_some)
 : hp₁.is_some :=
 sorry
 
-lemma is_some_of_is_some_part__left
+lemma is_some_of_is_some_part_left
   {hp₀ : option heap} (hp₁ : option heap)
-  (h : (part_ hp₀ hp₁).is_some)
+  (h : (part hp₀ hp₁).is_some)
 : hp₀.is_some :=
 sorry
 
@@ -93,28 +192,28 @@ lemma opt_apl_some (hp : heap) (p : pointer)
 : opt_apl (some hp) p = hp p :=
 rfl
 
-lemma opt_apl_part__maplet (hp : heap) (p : pointer) (v : word)
+lemma opt_apl_part_maplet (hp : heap) (p : pointer) (v : word)
   (h : maplet p v ## hp)
-: (opt_apl (part_ (some (maplet p v)) (some hp)) p) = some v :=
+: (opt_apl (part (some (maplet p v)) (some hp)) p) = some v :=
 begin
-  unfold part_,
+  unfold part,
   rw [dif_pos] ; [ skip , apply h ],
   rw [opt_apl,part',maplet,if_pos rfl],
   refl,
 end
 
 @[simp]
-lemma eq_emp_of_part_ (a : heap) (hp : option heap)
-: some a = part_ (some a) hp ↔ hp = some heap.emp :=
+lemma eq_emp_of_part (a : heap) (hp : option heap)
+: some a = part (some a) hp ↔ hp = some heap.emp :=
 sorry
 
 @[simp]
 lemma part'_eq_emp (a b : option heap)
-: part_ a b = some heap.emp ↔ a = some heap.emp ∧ b = some heap.emp :=
+: part a b = some heap.emp ↔ a = some heap.emp ∧ b = some heap.emp :=
 sorry
 
 def heap.le (hp₀ hp₁ : heap) : Prop :=
-∃ hp, some hp₁ = part_ (some hp₀) hp
+∃ hp, some hp₁ = part (some hp₀) hp
 
 instance : has_le heap :=
 ⟨ heap.le ⟩
@@ -126,12 +225,12 @@ instance : partial_order heap :=
                    simp [has_le.le,heap.le],
                    intros hp₀ h₀ hp₁ h₁,
                    -- have : hp₀ ## hp₁, admit,
-                   existsi part_ hp₀ hp₁,
+                   existsi part hp₀ hp₁,
                    simp [h₁,h₀], ac_refl }
 , le_antisymm := by { introv,
                       simp [has_le.le,heap.le],
                       intros hp₀ h₀ hp₁ h₁,
-                      simp [h₀,part__assoc] at h₁,
+                      simp [h₀,part_assoc] at h₁,
                       simp [h₁.left] at h₀,
                       subst b, }
 }
@@ -147,7 +246,7 @@ begin
     unfold has_le.le heap.le at h',
     cases h' with hp' h', cases hp' with hp',
     { contradiction },
-    have h₂ := eq_part'_of_some_eq_part_ _ _ _ h',
+    have h₂ := eq_part'_of_some_eq_part _ _ _ h',
     rw [h₂,part',maplet,if_pos h],
     simp },
   { simp [part', heap.delete, maplet, if_neg, h] }
